$$
\begin{align} 
\ln \frac{2x+1}{x+\sqrt{ x^{2}+1 }}\ge f(x) \ge 0 \\
\ln \frac{2x+1}{x+\sqrt{ x^{2}+1 }}-f(x) = F(x) \\
F(x)\ge 0 \\
\lim_{ x \to \infty } \ln \frac{2x+1}{x+\sqrt{ x^{2}+1 }}= \\
\lim_{ x \to \infty } \frac{\left( 2+\frac{1}{x} \right)}{1+\sqrt{ 1+\frac{1}{x^{2}} }} = 1 \\
\therefore \lim_{ x \to \infty } F(x) = 0; \\
F(x) = 0 when \ x=0; \\
\exists \xi>0,s.t.F(\xi) \ge 0; \\
\therefore \exists \alpha \in(0,\xi)s.t.F(\alpha)=\frac{F(\xi)}{2} \\

\therefore \exists \beta \in (\xi,\infty)s.t.F(\alpha)=\frac{F(\xi)}{2} \\ 
\therefore \exists \delta \in(\alpha,\beta)s.t.F'(x) = 0; \\
then \ f'(\delta) = \frac{2}{2\delta+1}-\frac{1}{\sqrt{ 1+\delta^{2} }}

\end{align} 

$$


$$
\begin{align}
&F(x) = f(x)-g(x) \\
 & F(a) = F(b)=0; \\
  & \because \sup f(x) = \sup g(x) \\
&\therefore \exists \alpha ,\beta\in(a,b)s.t.F(\alpha) > 0 ,F(\beta)>0; \\
 &\therefore  \exists \delta \in(\alpha,\beta)s.t.F(x) = 0; \\ 
 & \therefore \ \exists \xi_{1} \in(a,\delta),\xi_{2}\in(\delta,b)\ s.t.F'(\xi_{1}) = 0,F'(\xi_{2}) = 0 \\
 & \therefore  \exists \xi s.t.F'(\xi) = 0 \\
f''(\xi) = g''(\xi)
\end{align}
$$

$$\begin{align}
 & g''(x) \ne 0; \\
 & g''(x) >0 \\
 & if\ \exists x_{0}s.t.g(x) = 0; \\
 & \exists x_{1} ,x_{2},s.t.g'(x_{1}) = g'(x_{2}) = 0; \\
 & \exists x_{3} s.t.g''(x_{3})= 0; \\

 & \therefore \forall x\in(a,b),g(x)\ne 0 \\
 & (2) \\
 &  g''(c)f(c)-f''(c)g(c)= 0 \\
 & F(x) = \frac{f(x)}{g(x)} \\
 & F'(x) = \frac{f'(x)\cdot g(x)-f(x)g'(x)}{g^{2}(x)} \\
 & G(x)= f'(x)\cdot g(x)-f(x)g'(x) \\
 & G'(x)  =f''(x)\cdot g(x)+f'(x)\cdot g(x)-(f'(x)\cdot g'(x)+f(x)\cdot g''(x)) \\
& =f''(x)\cdot g(x)-f(x)\cdot g''(x) \\
  & G(a)=G(b)=0
\end{align}
$$
$$\begin{align}
 & (a+b\cos x)\sin x=(a-b(1-\cos x)+b)\sin x \\
 & =\left( (a+b)+b\left( \frac{x^{2}}{2}-\frac{x^{4}}{4!} \right) \right)\left( x-\frac{x^3}{3!} \right) \\
 & =(a+b)x+\frac{b}{2}x^{3}-\frac{b}{4!}x^{5}-\frac{a+b}{3!}x^{3}-
\end{align}
$$