$$
\begin{align}
&3\mathrm{B}-2 \\
&a)\sum_{i=1}^{6} (-1)^i(21+1) \\
&b)\sum_{i=1}^{n} \frac{1}{n^2} \\
&c)\sum_{i=1}^{n}{\sin \left( \frac{ix}{n} \right)} \\
&3\mathrm{B}-4 \\
&a)\int_{0}^1x^3 \mathrm{d}x  \\
 &upper:\lim_{ n \to \infty } \sum_{i=0}^{n}\left( \frac{1}{n} \right)\left( \frac{i}{n} \right)^3 \\
&lower:\lim_{ n \to \infty } \sum_{i=1}^{n}\left( \frac{1}{n} \right)\left( \frac{i-1}{n} \right)^3 \\
&b)\int_{-1}^{3}x^2\,\mathrm{d}x = \int_{-1}^{0}x^2\,\mathrm{d}x +\int_{0}^{3}x^2\,\mathrm{d}x \\
&upper:\lim_{ n \to \infty }\sum_{i=1}^{n} \left( \frac{1}{n} \right)\left( \frac{i}{n} \right)^2+\lim_{ n \to \infty }\sum_{i=1}^{n} \left( \frac{3}{n} \right)\left( \frac{3i}{n} \right)^2 \\
&lower:\lim_{ n \to \infty }\sum_{i=1}^{n} \left( \frac{1}{n} \right)\left( \frac{i-1}{n} \right)^2+\lim_{ n \to \infty }\sum_{i=1}^{n} \left( \frac{3}{n} \right)\left( \frac{3i-3}{n} \right)^2  \\
&c)\int_{0}^{2\pi}\sin x\, \mathrm{d}x = 0; \\ \\

 
\end{align}
$$

$$
\begin{align}
&3\mathbf{B}-5\\
&\lim_{ n \to \infty }\frac{\sum_{i=1}^{n}\sin \left( \frac{ib}{n} \right)}{n} =\int_{0}^{b}{\sin x}\,\mathrm{d}x=-\cos x|_{x=0}^{x=b}=-\cos b-(-\cos 0)=1-\cos b
\end{align}

$$
$$
\begin{align} \\
3\mathbf{B}-6^* \\
&Calculate\int_{0}^{1}e^x\,\mathrm{d}\ by\  using\ upper\ Riemann\ Sums \\
&upper RS = \lim_{ n \to \infty }\sum_{i=1}^{n}\frac{e^{\frac{i}{n}}}{n}  \\
&=\lim_{ n \to \infty } \frac{1}{n}\sqrt[n]{e }\frac{1-e^{\frac{n+1}{n}}}{1-\sqrt[n]{ e }}=e-1

\end{align} \\

$$
